Statements.fst
@@ -1,6 +1,20 @@
 module Statements
 
-open Reforge
+open Solidity
+
+(*
+        Statement01: Overflow in `_mint` function is not possible in the `unchecked` part (of soliditxy code)
+        
+        Proof is trivial, since we have alerady shown that 
+        updated_totalSupply >= updated_balances[account] `assertion (_totalSupply >= updated _balances[account])`, and 
+        that increase of _totalSupply didn't result in overflow `overflow_check and match`,
+        thus it logically implies that _accountBalance_upd has not overlowed!
+*)
+let lemma_overflow_impossible (_totalSupply_upd:uint) (_accountBalance_upd:uint) : Lemma 
+                                        (requires   ((FStar.UInt256.lte _totalSupply_upd Solidity.max_uint) /\
+                                                     (FStar.UInt256.gte _totalSupply_upd _accountBalance_upd)))
+                                        (ensures  (FStar.UInt256.lte _accountBalance_upd Solidity.max_uint)) 
+                                        = ()
 
 (*	    Statement01: Global state reamins valid after refogrge *)
 // TODO
